Notation + example
4+5-2*3 = 3

ae_compiler.v
@@ -1,4 +1,4 @@
-Require Import bf_stack bf.
+Require Import bf_stack bf bf_semantics.
 
 Inductive ae : Set :=
 | Int : nat -> ae
@@ -6,12 +6,19 @@ Inductive ae : Set :=
 | Minus : ae -> ae -> ae
 | Mult : ae -> ae -> ae.
 
-Fixpoint interpret ae : nat :=
+Coercion Int : nat >-> ae.
+Notation "a + b" := (Plus a b) : ae_scope.
+Notation "a - b" := (Minus a b) : ae_scope.
+Notation "a * b" := (Mult a b) : ae_scope.
+
+Open Scope ae_scope.
+
+Fixpoint interpret (ae : ae) : nat :=
   match ae with
     | Int n => n
-    | Plus e1 e2 => interpret e1 + interpret e2
-    | Minus e1 e2 => interpret e1 - interpret e2
-    | Mult e1 e2 => interpret e1 * interpret e2
+    | Plus e1 e2 => (interpret e1 + interpret e2)%nat
+    | Minus e1 e2 => (interpret e1 - interpret e2)%nat
+    | Mult e1 e2 => (interpret e1 * interpret e2)%nat
   end.
 
 Fixpoint compile (ae : ae) : Instr.instruction :=
@@ -21,5 +28,15 @@ Fixpoint compile (ae : ae) : Instr.instruction :=
     | Minus e1 e2 => compile e1; compile e2; sub
     | Mult e1 e2 => compile e1; compile e2; mult
   end.
+
+Example interpret_compile_example1 :
+  iter (compile (4+5-2*3), init zeroes)
+       (END, state[zeroes, interpret (4+5-2*3), zeroes, zeroes, nil]).
+Proof.
+  unfold init, compile, interpret.
+  repeat bf_step.
+  unfold sub.
+  repeat bf_step.
+Qed.
 
 (* TODO: Correctness proof *)
